cem.v
@@ -1,6 +1,6 @@
 Require Import db util.
 Require Import Arith.EqNat.
-Require Import List Unicode.Utf8 Arith.Peano_dec.
+Require Import List Unicode.Utf8 Arith.Peano_dec Basics.
 Require Import CpdtTactics.
 
 Definition append := Datatypes.app.
@@ -17,8 +17,10 @@ Definition clclose (c: cell) : closure := match c with cl c e => c end.
 
 Definition heap := Map nat cell.
 
-Inductive configuration : Type :=
-  | conf : heap → closure → configuration.
+Record configuration : Type := conf {
+  st_heap : heap;
+  st_clos : closure
+}.
 
 Definition I (e : tm) : configuration := conf nil (close e 0).
 
@@ -44,9 +46,6 @@ Fixpoint clu (v env:nat) (h:heap) : option (nat * closure) := match lookup env h
     end
   end.
 
-Definition isfresh (h : heap) (n : nat) : Prop := ¬ In n (domain h). 
-Axiom fresh : ∀ h:heap, @sig nat (isfresh h). 
-
 Definition closed_under (c : closure) (h : heap)  : Prop := match c with
   | close t e => forevery (fvs t) 
       (λ x, ∃e' c', clu x e h = Some (e',c') ∧ In e' (domain h))
@@ -58,7 +57,7 @@ Definition well_formed_heap (h : heap) : Prop := forevery h
   (λ x, match x with | (v,cl c e') => closed_under c h end). 
 
 Definition well_formed (c : configuration) : Prop := match c with 
-  | conf h t => closed_under t h ∧ well_formed_heap h 
+  | conf h t => closed_under t h ∧ well_formed_heap h ∧ unique (domain h)
   end.
 
 Reserved Notation " c1 '⇓' c2 " (at level 50).
@@ -67,8 +66,8 @@ Inductive step : configuration → configuration → Prop :=
             ⟨Φ, (x ↦ {M,y}), Υ⟩M ⇓ ⟨Ψ, (x ↦ {M,y}), Υ⟩close (:λB) e →
     ⟨Φ, x ↦ {M, y}, Υ⟩close (var v) z ⇓ ⟨Ψ, x ↦ {close (:λB) e, y}, Υ⟩close (:λB) e
   | Abs : ∀ N Φ e, ⟨Φ⟩close (:λN) e ⇓ ⟨Φ⟩close (:λN) e
-  | App : ∀ N M B B' Φ Ψ Υ f e ne ae p, 
-                fresh Ψ = exist (isfresh Ψ) f p → 
+  | App : ∀ N M B B' Φ Ψ Υ f e ne ae, 
+                  fresh' f Ψ → 
           ⟨Φ⟩close M e ⇓ ⟨Ψ⟩close (:λB) ne → 
       ⟨Ψ, f ↦ {close N e, ne}⟩close B f ⇓ ⟨Υ⟩close (:λB') ae   →
               ⟨Φ⟩close (M@N) e ⇓ ⟨Υ⟩close (:λB') ae
@@ -81,68 +80,143 @@ Definition step' (c1 c2: configuration') : Prop := match (c1, c2) with
 Lemma well_formed_inf : ∀ c x c' n  Φ Υ, 
   well_formed (⟨Φ, x ↦ cl c' n, Υ⟩c) → 
   well_formed (⟨Φ, x ↦ cl c' n, Υ⟩c').
-intros. split. inversion H. unfold well_formed_heap in H1. apply forevery_app in H1.
-destruct H1. simpl in H2. destruct H2. auto. 
-auto. inversion H. auto. Qed. 
+intros. split. inversion H. destruct H1. unfold well_formed_heap in H1. apply
+forevery_app in H1.  destruct H1. simpl in H3. destruct H3. auto. split;
+destruct H; destruct H0; auto. Qed.
 
 Lemma forevery_cons {A} : ∀ (p:A→Prop) (x:A) xs, p x → forevery xs p → forevery (x::xs) p. 
 intros. simpl. split; assumption. Qed. 
 
-(*
+Lemma clu_inf : ∀ x x' c c' e e'  Ψ Φ clo n, 
+  clu x e (Φ ++ x' ↦ cl c e' :: Ψ) = Some (n, clo) →
+  ∃ clo', clu x e (Φ ++ x' ↦ cl c' e' :: Ψ) = Some (n, clo').
+intros x. induction x. intros. simpl in H. remember (lookup e (Φ ++ x' ↦ cl c e' :: Ψ)).
+simpl. destruct o. symmetry in Heqo. apply (ex_intro (λ x, lookup e (Φ ++ x' ↦ cl
+c e' :: Ψ) = Some x) c0) in Heqo. apply lookup_in_domain in Heqo. rewrite
+domain_inf with (m':= cl c' e') in Heqo. apply in_domain_lookup in Heqo.
+destruct Heqo. rewrite H0. destruct x. destruct c0. inversion H. subst. clear H.
+exists c1. reflexivity. inversion H. intros. specialize (IHx x' c c').
+simpl in H. remember (lookup e (Φ ++ x' ↦  cl c e' :: Ψ)). destruct o.  destruct
+c0. specialize (IHx n0 e' Ψ Φ clo n H). destruct IHx. simpl. remember (lookup e (Φ ++
+x' ↦ cl c' e' :: Ψ)). destruct o. destruct c1. assert (n1 = n0). clear H0. clear
+H. induction Φ.  simpl in Heqo. simpl in Heqo0. unfold lookup in Heqo. unfold
+lookup in Heqo0.  simpl in Heqo. simpl in Heqo0. destruct (beq_nat e x').
+inversion Heqo. subst.  inversion Heqo0. subst. reflexivity. rewrite <- Heqo in
+Heqo0.  inversion Heqo0.  subst. reflexivity. destruct a. unfold lookup in Heqo.
+unfold lookup in Heqo0. simpl in Heqo. simpl in Heqo0. destruct (beq_nat e n2). 
+rewrite <- Heqo in Heqo0. inversion Heqo0. subst. reflexivity. simpl in Heqo.
+simpl in Heqo0. apply IHΦ. assumption. assumption. subst. exists x0. assumption. symmetry
+in Heqo. apply (ex_intro (λ x, lookup e (Φ ++ x' ↦ cl c e' :: Ψ) = Some x) (cl
+c0 n0)) in Heqo. apply lookup_in_domain in Heqo. rewrite domain_inf with (m':=cl
+c' e') in Heqo. apply in_domain_lookup in Heqo. destruct Heqo. rewrite H1 in
+Heqo0. inversion Heqo0. inversion H. Qed. 
 
-Lemma closed_under_inf' : ∀ c c' e x Ψ Φ, closed_under c (Φ ++ x ↦ {c', e} :: Ψ) →
-  closed_under c (Φ ++ x ↦ {c, e} :: Ψ).
-intros. unfold closed_under. destruct c. unfold closed_under in H. induction (fvs clos_tm0). simpl. auto.
-simpl. split. simpl in H. destruct H. destruct H. destruct H. destruct H.
-destruct (clu a clos_env0 (Φ ++ x ↦ {c', e} :: Ψ)). destruct p. inversion H.
-destruct c. destruct = 
-destruct H. 
-apply
-ex_intro with x0. apply ex_intro with x1. split. destapply forevery_inf with (xs:=Φ)
-(ys:=Ψ) (y:=x ↦ {, e}). . .  forevery_app in H. 
+Lemma closed_under_inf' : ∀ c c' c'' e x Ψ Φ, closed_under c (Φ ++ x ↦ {c', e} :: Ψ) →
+  closed_under c (Φ ++ x ↦ {c'', e} :: Ψ).
+intros. unfold closed_under. unfold closed_under in H. destruct c.  
+apply forevery_impl with (p:=(λ x0 : nat,
+       ∃ (e' : nat) (c'0 : closure),
+       clu x0 clos_env0 (Φ ++ x ↦ {c', e} :: Ψ) = Some (e' ↦ c'0)
+       ∧ In e' (domain (Φ ++ x ↦ {c', e} :: Ψ)))). 
+intros. destruct H0. destruct H0. destruct H0. apply clu_inf with
+(c':=c'') in H0. destruct H0. destruct x2. exists x0, (close
+clos_tm1 clos_env1). split. assumption.  rewrite domain_inf with (m':=cl c' e).
+assumption. assumption. Qed.
 
 Lemma well_formed_inf' : ∀ Φ Ψ x c c' n,
   well_formed (⟨Φ, x ↦ cl c' n, Ψ⟩c) →
   well_formed (⟨Φ, x ↦ cl c n, Ψ⟩c).
-intros. split.  inversion H. apply forevery_app in H1. destruct H1. simpl in H2. destruct H2. rename x into X. apply forevery_cons
-with (x:=X ↦ {c', n}) (xs:=Φ) in H0. assumption. apply  . assumption.  in H0. assert (conj H0 H3). forevery (x ↦ {c, n} :: Φ), λ
-x0, match x0 with _ ↦ {c1, _} => closed_under c1 (append (nat * cell) Ψ (x ↦ {c',
-n} :: Φ)) end). 
-unfold closed_under. rewrite forevery_app.  with (m:=n) (m':=n). assumption.
-unfold well_formed_heap. unfold closed_under.  unfold well_formed_heap in H0.
-unfold closed_under in H0. rewrite domain_inf with (m:=N) (m':=M). rewrite
-forevery_app. rewrite forevery_app in H0. destruct H0. split. crush. crush. 
-Qed.
+intros. split.  inversion H. apply closed_under_inf' with (c':=c'). assumption.
+split. destruct H. destruct H0. apply forevery_app in H0. destruct H0. simpl in H2.
+destruct H2. rename x into X. apply forevery_cons with (x:=X ↦ {c, n}) (xs:=Φ)
+in H3; try assumption. assert (h' := conj H0 H3). rewrite <- forevery_app in h'.
+clear H3 H0. apply forevery_impl with (p:=(λ x : nat * cell,
+        let (_, c0) := x in
+        match c0 with
+        | {c1, _} =>
+            closed_under c1 (append (nat * cell) Ψ (X ↦ {c', n} :: Φ))
+        end)).
+intros.
+destruct a. destruct c0. apply closed_under_inf' with (c':=c'). assumption.
+assumption. destruct H. destruct H0. rewrite domain_inf with (m':=cl c' n).
+assumption. Qed.
 
-TODO
-Lemma cactus_lookup_inf : ∀ v x y m n e Φ Υ, cactus_lookup v x (Φ ++ (y ↦ {m, n}) :: Υ) e → ∀ M, cactus_lookup v x (Φ ++ (y ↦ {M, n}) :: Υ) e.
-intros. 
+Lemma clu_cons : ∀ c c' x ne ne' xs f,
+  fresh' f xs →
+  clu x ne xs = Some c → 
+  clu x ne (f↦cl c' ne'::xs) = Some c.
+intros c c' x. induction x; intros. simpl in H0. remember (lookup ne xs). destruct
+o. destruct c0. symmetry in Heqo. assert (lu:=Heqo). apply (ex_intro (λ x, lookup ne xs = Some x)
+(cl c0 n)) in Heqo. simpl. unfold lookup. simpl. destruct (eq_nat_dec ne f).
+subst. apply lookup_in_domain in Heqo. apply H in Heqo. inversion Heqo. rewrite
+<- beq_nat_false_iff in n0. rewrite n0.  unfold lookup in lu. rewrite lu.
+assumption. inversion H0. destruct (eq_nat_dec ne f). subst. simpl in H0.
+remember (lookup f xs). destruct o. symmetry in Heqo. assert (lu:=Heqo). apply
+(ex_intro (λ x, lookup f xs = Some x) c0) in Heqo. apply lookup_in_domain in
+Heqo. apply H in Heqo. inversion Heqo. inversion H0. simpl. unfold lookup.
+rewrite <- beq_nat_false_iff in n. simpl. rewrite n. simpl in H0. unfold lookup
+in H0. destruct (find (λ p : nat * cell, beq_nat ne (fst p)) xs). destruct p.
+destruct c0. apply IHx. assumption. assumption. inversion H0. Qed.
 
-Lemma inf_well_formed : ∀ c x c' n  Φ Υ, well_formed (⟨Φ, x ↦ cl c' n, Υ⟩c) → 
-  well_formed (⟨Φ, x ↦ cl c n, Υ⟩c).
-  intros. inversion H. split. induction Υ. simpl. destruct c. induction (fvs e).
-  simpl. auto. simpl. 
-  destruct (eq_nat_dec x n0). simpl. unfold domain. rewrite
-  map_app. simpl. unfold domain in H0. rewrite map_app in H0. simpl in H0. 
-  kapply forevery_app in H1. destruct H1. simpl in
-  H2. destruct H2. unfold closed_under in H0. clear H1 H2 H3.  (inversion H. apply forevery_app in H1.
-  auto. inversion H. auto. Qed. 
+Lemma clu_monotonic : ∀ Φ Ψ x e c v l cl, 
+  clu x e Φ = Some (l,cl) →
+  ⟨Φ⟩c ⇓ ⟨Ψ⟩v  →
+  ∃ cl', clu x e Ψ = Some (l, cl').
+intros. remember (conf Φ c). remember (conf Ψ v). generalize dependent c.
+generalize dependent v. generalize dependent l. generalize dependent cl0.
+generalize dependent x. generalize dependent Φ. generalize dependent Ψ.
+generalize dependent e. induction H0; intros. inversion Heqc0. inversion
+Heqc1. subst. specialize (IHstep e0 (Υ ++ x ↦ {M, y} :: Ψ) (Υ ++
+x ↦ {M, y} :: Φ) x0 cl0 l H1 (close (lam B) e) eq_refl M eq_refl). destruct
+IHstep. apply clu_inf with (c':=close (lam B) e) in H2. assumption. 
+inversion Heqc1. inversion Heqc0. subst. inversion Heqc0. subst. exists cl0.
+assumption. inversion Heqc1. subst. inversion Heqc0. subst. clear Heqc1. clear
+Heqc0. apply IHstep1 with (Ψ0:=Ψ)(v:=close (lam B) ne) (c:= close M e) in
+H0; try reflexivity. destruct H0. apply IHstep2 with (Φ:=f↦(cl (close N e)
+ne)::Ψ) (cl0:=x0) (c:=close B f) (v:=close (lam B') ae). apply clu_cons.
+assumption. assumption. reflexivity. reflexivity. Qed. 
+
+Lemma monotonic_heap : ∀ c1 c2, c1 ⇓ c2 → domain (st_heap c1) ⊆ domain (st_heap c2).  
+intros c1 c2 step.  induction step. simpl. simpl in IHstep. 
+unfold domain at 2. unfold domain at 2 in IHstep. rewrite map_app. rewrite
+map_app in IHstep.  simpl. simpl in IHstep. assumption. 
+apply subset_id. simpl. simpl in IHstep1. simpl in IHstep2. destruct IHstep2. 
+apply subset_trans with (ys:=domain Ψ). assumption. assumption. Qed.
 
 Theorem well_formed_step : ∀ c v, well_formed c → c ⇓ v → well_formed v.
 intros. induction H0. apply well_formed_inf in H. apply IHstep in H.  
-
+apply well_formed_inf' in H. assumption. assumption. apply IHstep2. destruct H.
+simpl in H. apply forevery_app in H. destruct H. specialize (IHstep1 (conj H
+H1)). split; try split. clear H H2 H1 IHstep2 H0_ H0_0. destruct IHstep1.
+destruct H1. simpl. simpl in H. rewrite forevery_map in H. induction (fvs B).
+simpl.  auto. destruct a. simpl in H. apply IHl in H. simpl. split; try
+assumption.  unfold lookup. simpl. rewrite <- beq_nat_refl. exists f, (close N
+e). split; auto. simpl. simpl in H. destruct H. split; try (apply IHl;
+assumption). unfold compose in H. simpl in H.  unfold lookup. simpl. rewrite <-
+beq_nat_refl.  destruct H. destruct H. exists x , x0. destruct H. split; auto.
+apply clu_cons; assumption. unfold well_formed_heap. simpl. split. apply
+forevery_impl with (p:=(λ x : nat,
+        ∃ (e' : nat) (c' : closure),
+        clu x e Φ = Some (e' ↦ c') ∧ In e' (domain Φ))). 
+intros. destruct H3.
+destruct H3. destruct H3.  apply (clu_monotonic Φ Ψ a e (close M e)
+(close (lam B) ne) x x0) in H3. destruct H3. exists x, x1. split. apply
+clu_cons.  assumption. assumption. apply or_intror. apply monotonic_heap
+in H0_. simpl in H0_. rewrite <- subset_eq in H0_. apply H0_ in H4.
+assumption. assumption. assumption. inversion IHstep1. destruct H4. unfold
+well_formed_heap in H4. apply forevery_impl with (p:= (λ x : nat * cell,
+        let (_, c0) := x in match c0 with
+                            | {c, _} => closed_under c Ψ
+                            end)). 
+intros. destruct a. destruct c. unfold closed_under. destruct c. unfold
+closed_under in H6. apply forevery_impl with (p:=(λ x : nat,
+        ∃ (e' : nat) (c' : closure),
+        clu x clos_env0 Ψ = Some (e' ↦ c') ∧ In e' (domain Ψ))).
+intros. destruct H7. destruct H7. destruct H7. exists x, x0. split. apply
+clu_cons; assumption. simpl. auto. assumption. assumption. apply ucons. simpl.
+destruct H0.  assumption. destruct IHstep1. destruct H4. unfold domain in H5.
+assumption. Qed. 
+    
 Lemma values_only : ∀ c e M Ψ, c ⇓ ⟨Ψ⟩close M e → value M.
-intros. inversion H; simpl; auto. Qed.
+intros. inversion H; simpl; constructor. Qed.
 
-Example simple : (step (⟨nil⟩ close (:λ0 @ :λ0) 0) (⟨nil, 0 ↦ {close (:λ0) 0,
-0}⟩ close (:λ0) 0)).
-apply App with 0 nil 0 0.
-unfold fresh. simpl.  auto. 
-apply Abs.
-rewrite <- app_nil_l with (prod nat cell) (cons (0↦{close (:λ0) 0, 0}) nil).
-apply Id.
-apply zero.
-apply Abs. 
-Qed.
-
-*)
